Add VST spec for encoder/decoder

src/PrimitiveDecoder/BooleanVSTSpec.v
@@ -1,14 +1,151 @@
 (* VST specification of as *)
 Require Import Clight.asn_codecs_prim.
 Require Import Core.Core Lib.
-Require Import VST.floyd.proofauto.
+Require Import VST.floyd.proofauto Psatz.
 Require Import BooleanExecSpec.
+Require Import ErrorWithWriter.
 
 Definition Vprog : varspecs. mk_varspecs prog. Defined.
 Instance CompSpecs : compspecs. make_compspecs prog. Defined.
 
 Open Scope Z.
 
-Section PrimitiveParser.
+Section Boolean_der_encode_primitive.
 
-End PrimitiveParser.
+Definition cb_type := (Tfunction 
+                          (Tcons (tptr tvoid) 
+                                 (Tcons tuint (Tcons (tptr tvoid) Tnil))) tint 
+                          cc_default).
+
+Definition bool_der_encode_primitive_spec : ident * funspec :=
+  DECLARE _der_encode_primitive
+    WITH (* pointer to the decoded structure *)
+         sptr_b : block, sptr_ofs : ptrofs, sptr_val : Z, sh_sptr : share,
+         (* pointer to the DEF table for the type decoded *)
+         td_b : block, td_ofs : ptrofs, sh_td : share,
+         td : TYPE_descriptor,
+         tag_mode : Z, tag_class : Z,
+         (* callback pointer *)
+         cb_b : block, cb_ofs : ptrofs, cb_val : val, sh_cb : share,
+         (* callback argument pointer *)
+         app_key_b : block, app_key_ofs : ptrofs,
+         app_key_val : val, sh_app_key : share
+    PRE  [         
+      (* added by clightgen - since returning structs is not supported *) 
+          __res OF (tptr (Tstruct _asn_enc_rval_s noattr)),
+          _td OF (tptr (Tstruct _asn_TYPE_descriptor_s noattr)),
+          _sptr OF (tptr tvoid), _tag_mode OF tint,
+          _tag OF tuint,
+          _cb OF (tptr cb_type),
+          _app_key OF (tptr tvoid)
+           ]
+    PROP ( readable_share sh_td;
+           writable_share sh_sptr; 
+           readable_share sh_cb;
+           readable_share sh_app_key )
+    LOCAL ( temp _td (Vptr td_b td_ofs);
+            temp _sptr (Vptr sptr_b sptr_ofs);
+            temp _tag_mode (Vint (Int.repr tag_mode));
+            temp _tag (Vint (Int.repr tag_class));
+            temp _cb (Vptr cb_b cb_ofs);
+            temp _app_key (Vptr app_key_b app_key_ofs))        
+    SEP ((* td points to td with readable permission *)
+           data_at sh_td (Tstruct _asn_TYPE_descriptor_s noattr) 
+                   (TYPE_descriptor_rep td) (Vptr td_b td_ofs) ; 
+           data_at sh_sptr (tvoid) (tt) (Vptr sptr_b sptr_ofs) ;
+           data_at sh_app_key (tvoid) (tt) 
+                   (Vptr app_key_b app_key_ofs) ;
+           data_at sh_cb (cb_type) (tt) (Vptr cb_b cb_ofs))
+    POST [tvoid]
+      PROP()
+      LOCAL ()
+      SEP( (* Unchanged by the execution : *)
+           data_at sh_td (Tstruct _asn_TYPE_descriptor_s noattr) 
+                   (TYPE_descriptor_rep td) (Vptr td_b td_ofs) ; 
+           data_at sh_sptr (tvoid) (tt) (Vptr sptr_b sptr_ofs) ;
+           data_at sh_app_key (tvoid) (tt) 
+                   (Vptr app_key_b app_key_ofs) ;
+           data_at sh_cb (cb_type) (tt) (Vptr cb_b cb_ofs)).
+
+Definition Gprog1 := ltac:(with_library prog [bool_der_encode_primitive_spec]).
+
+Theorem bool_der_encode : semax_body Vprog Gprog1 f_der_encode_primitive
+                                     bool_der_encode_primitive_spec.
+Admitted.
+
+End Boolean_der_encode_primitive.
+
+Section Boolean_der_decode_primitive.
+
+Definition bool_ber_decode_primitive_spec : ident * funspec :=
+  DECLARE _ber_decode_primitive
+    WITH (* pointer to the decoded structure *)
+         sptr_b : block, sptr_ofs : ptrofs,
+         (* double pointer to the DEF table for the type decoded *)
+         td_b : block, td_ofs : ptrofs,
+         td'_b : block, td'_ofs : ptrofs,
+         (* pointer to  the input buffer *)
+         buf_b : block, buf_ofs : ptrofs,
+         (* pointer to the return struct dec_rval *)                         
+         res_b : block, res_ofs : ptrofs,
+         (* codec context: stores max_stack_size for the decoder routines *)
+         ctx : val,
+         (* memory permissions for each pointer *)
+         sh_sptr : share, sh_td : share, sh_buf : share, sh_td' : share,
+         sh_res : share,                                                         
+         (* input *)
+         buf : list byte,
+         td : TYPE_descriptor,
+         size : int,
+         tag_mode : int  
+    PRE  [         
+ (* added by clightgen - since returning structs is not supported *) 
+          __res OF (tptr (Tstruct _asn_dec_rval_s noattr)),
+          _opt_codec_ctx OF (tptr (Tstruct _asn_codec_ctx_s noattr)),
+          _td OF (tptr (Tstruct _asn_TYPE_descriptor_s noattr)),
+          _sptr OF (tptr (tptr tvoid)),
+          _buf_ptr OF (tptr tvoid),
+          _size OF tuint,
+          _tag_mode OF tint ]
+    PROP ( writable_share sh_sptr; 
+           writable_share sh_res; 
+           readable_share sh_td;
+           readable_share sh_buf )
+    LOCAL ( temp _opt_codec_ctx ctx;
+            temp _td (Vptr td_b td_ofs);
+            temp _sptr (Vptr sptr_b sptr_ofs);
+            temp _buf_ptr (Vptr buf_b buf_ofs);
+            temp _size (Vint size);
+            temp _tag_mode (Vint tag_mode))        
+    SEP ((* td points to td with readable permission *)
+           data_at sh_td (tptr (Tstruct _asn_TYPE_descriptor_s noattr)) 
+                   (Vptr td'_b td'_ofs) (Vptr td_b td_ofs);
+           data_at sh_td' (Tstruct _asn_TYPE_descriptor_s noattr) 
+                   (TYPE_descriptor_rep td) (Vptr td'_b td'_ofs) ; 
+           (* buf points to data ls *)
+           data_at sh_buf (tarray tschar (Zlength buf)) (map Vbyte buf) 
+                   (Vptr buf_b buf_ofs))
+    POST [tvoid]
+      PROP()
+      LOCAL ()
+      SEP( (* Unchanged by the execution : *)
+           data_at sh_td (tptr (Tstruct _asn_TYPE_descriptor_s noattr)) 
+                   (Vptr td'_b td'_ofs) (Vptr td_b td_ofs);
+           data_at sh_td' (Tstruct _asn_TYPE_descriptor_s noattr) 
+                   (TYPE_descriptor_rep td) (Vptr td'_b td'_ofs) ; 
+           data_at sh_buf (tarray tschar (Zlength buf)) (map Vbyte buf) 
+                   (Vptr buf_b buf_ofs);
+           (* Changed after execution *)         
+           data_at sh_sptr (Tstruct _ASN__PRIMITIVE_TYPE_s noattr)
+                   (PRIMITIVE_TYPE_rep (bool_prim_decoder td buf))
+                                       (Vptr sptr_b sptr_ofs); 
+           data_at sh_res (Tstruct _asn_dec_rval_s noattr)
+                   (dec_rval_rep (bool_prim_decoder td buf)) (Vptr res_b res_ofs)).
+
+Definition Gprog2 := ltac:(with_library prog [bool_ber_decode_primitive_spec]).
+
+Theorem bool_ber_decode : semax_body Vprog Gprog2 f_ber_decode_primitive
+                                     bool_ber_decode_primitive_spec.
+Admitted.
+
+End Boolean_der_decode_primitive.
