src/PrimitiveDecoder/Lib.v
@@ -2,6 +2,7 @@ From Coq Require Import String.
 Require Import Core.Core.
 Require Import VST.floyd.proofauto.
 Require Import Clight.asn_codecs_prim.
+Require Import ExtLib.Structures.Monad.
 
 Instance CompSpecs : compspecs. make_compspecs prog. Defined.
 
@@ -29,9 +30,9 @@ Parameter TYPE_descriptor_rep : TYPE_descriptor
 
 (* on any error write {buf = 0; size = 0},
     else {buf = ls; size = |ls|}*)
-Parameter PRIMITIVE_TYPE_rep : option (list byte) 
+Parameter PRIMITIVE_TYPE_rep : option byte
                                -> reptype (Tstruct _ASN__PRIMITIVE_TYPE_s noattr).
 
 (* on error rval c l write {code := c; consumed := l},
    else {code := OK; consumed := |ls| *)
-Parameter dec_rval_rep : option (list byte) -> reptype (Tstruct _asn_dec_rval_s noattr).
+Parameter dec_rval_rep : option byte -> reptype (Tstruct _asn_dec_rval_s noattr).
